%% LyX 2.3.7 created this file.  For more info, see http://www.lyx.org/.
%% Do not edit unless you really know what you are doing.
\documentclass[english]{amsart}
\usepackage[T1]{fontenc}
\usepackage[latin9]{inputenc}
\usepackage{amstext}
\usepackage{amsthm}

\makeatletter
%%%%%%%%%%%%%%%%%%%%%%%%%%%%%% Textclass specific LaTeX commands.
\numberwithin{equation}{section}
\numberwithin{figure}{section}

\makeatother

\usepackage{babel}
\begin{document}
E-L equation proof

\begin{abstract}
Abstract: find a function x(t) that extremizes the functional L. 
\end{abstract}

let x(t) be the functino that extremizes the functional L(x(t)) =
$\int x(t)d$. Let A(t) be the function that represents the divigergence
from the idealized path x(t). Let $A(t_{1})=A(t_{2})=0$. All possible
paths can be represented by x(t,a) = x(t) + aA(t) where a parameterizes
the divergence of the path. 

let L(a) = $\int_{t_{1}}^{t_{2}}f(x(t,a),\dot{x}(t,a),t)dt$ be functional
parameterized by a. 

Note when a = 0 $\frac{dL}{da}$=0. 

$\frac{dL}{da}=\frac{d}{da}\int_{t_{1}}^{t_{2}}f(x(t,a),\dot{x}(t,a),t)dt$

$0=\int_{t_{1}}^{t_{2}}\frac{\text{\ensuremath{\partial f}}}{\partial x}\frac{\partial x}{\partial a}+\frac{\text{\ensuremath{\partial f}}}{\partial\dot{x}}\frac{\partial\dot{x}}{\partial a}dt$

\begin{align*}
\frac{\partial x}{\partial a} & =A(t)\\
\frac{\partial\dot{x}}{\partial a} & =\frac{\partial x}{\partial a}\times\frac{d}{dt}=A'(t)
\end{align*}

\[
0=\int_{t_{1}}^{t_{2}}\frac{\text{\ensuremath{\partial f}}}{\partial x}\cdot A(t)+\frac{\text{\ensuremath{\partial f}}}{\partial\dot{x}}\cdot A'(t)
\]

Using Integration by parts: 
\begin{align*}
\int\frac{\text{\ensuremath{\partial f}}}{\partial\dot{x}}\cdot A'(t)dt & =\frac{\partial f}{\partial\dot{x}}A(t)\Vert_{t_{1}}^{t_{2}}-\int\frac{d}{dt}\cdot\frac{\text{\ensuremath{\partial f}}}{\partial\dot{x}}*A(t)dt\\
 & =-\int\frac{d}{dt}\cdot\frac{\text{\ensuremath{\partial f}}}{\partial\dot{x}}*A(t)dt
\end{align*}

Thus
\begin{align*}
0 & =\int_{t_{1}}^{t_{2}}\frac{\text{\ensuremath{\partial f}}}{\partial x}\cdot A(t)-\frac{d}{dt}\frac{\text{\ensuremath{\partial f}}}{\partial\dot{x}}\cdot A(t)dt\\
 & =\int A(t)\cdot(\frac{\partial f}{\partial x}-\frac{d}{dt}\cdot\frac{\partial f}{\partial\dot{x}})dt
\end{align*}

As $A(t)$ is arbitrary everywhere on the interval 
\begin{align*}
\frac{\partial f}{\partial x}-\frac{d}{dt}\cdot\frac{\partial f}{\partial\dot{x}} & =0\\
\frac{d}{dt}\cdot\frac{\partial f}{\partial\dot{x}} & =\frac{df}{dx}
\end{align*}

proving Euler's equation. This equation must be satisfied for a function
x(t) that extremizes the functional L. 

\section*{Arc-Length}

Find the function x(t) that extremizes the functional 
\[
S=\int\sqrt{1-(\frac{dx}{dt})^{2}}dt
\]

This is the functional that calculates the arc length of a given path.
\begin{align*}
\frac{d}{dt}\cdot\frac{\partial f}{\partial\dot{x}} & =\frac{df}{dx}\\
\frac{d}{dt}\frac{-\dot{x}}{\sqrt{1-(\dot{x})^{2}}}=0\\
\frac{-\ddot{x}\sqrt{1-(\dot{x})^{2}}+\dot{x}^{2}\ddot{x}(1-\dot{x})^{-\frac{1}{2}}}{1-(\dot{x})^{2}}=0\\
\frac{\ddot{x}}{(1-\ddot{x}^{2})^{\frac{3}{2}}}=0
\end{align*}

Thus 
\begin{align*}
\ddot{x} & =0\\
\int\int\ddot{x}dt & =\int\int0\,dt\\
x & =mt+b
\end{align*}

Proving the shortest distance between two points is a straight line. 

Spring pendulum

\[
U=mg(l+x)cos(\theta)+\frac{1}{2}kx^{2}
\]

The Kinetic energy of the system is the linear kinetic energy of the
spring and the tangential Kinetic energy. 

\[
K=\frac{1}{2}m\dot{x}^{2}+\frac{1}{2}m(l+x)^{2}\dot{\theta}^{2}
\]

These energies are combined to make the Lagraganian
\[
L=K+U
\]

Let f(x) be the function that extremizes the action and thus is the
actual motion of the ball linearly. 

To find the function f(x) the following equation must be satisfied:
\begin{align*}
\frac{d}{dt}\frac{dL}{d\dot{x}} & =\frac{dL}{dx}\\
m\ddot{x} & =-mgsin(\theta)+kx+m(l+x)\dot{\theta}^{2}
\end{align*}

The RHS is the ma part of Newtons second law and the LHS is the gravitational
tangential force, the spring force, and the centrifugal force. 

Solving this, gives f(x). 

\[
\frac{d}{dt}\frac{dL}{d\dot{\theta}}=\frac{dL}{d\theta}
\]

\[
m(l+x)^{2}\ddot{\theta}=-mg(l+x)sin(\theta)
\]

This equation reveals that $\text{mass}$ $\times$tangential acceleration
= torque
\end{document}
